Util.v
@@ -8,13 +8,21 @@ Miscellaneous definitions and lemmas extending the Coq standard library.
 Set Implicit Arguments.
 
 Require Import ZArith.
-Require Import Coqlib. (*FIXME: needed for defining zne with Z_eq_dec*)
+Require Import Bool.
 
-Definition zne (x y : Z) : bool := negb (Z_eq_dec x y).
+Open Scope Z_scope.
+
+(****************************************************************************)
+
+Definition zne (x y : Z) : bool := if Z_eq_dec x y then false else true.
+
+(****************************************************************************)
 
 Notation beq := eqb.
 
 Definition bne (x y : bool) : bool := negb (eqb x y).
+
+(****************************************************************************)
 
 Lemma between_dec : forall a x b, {a <= x <= b}+{~(a <= x <= b)}.
 
@@ -23,6 +31,8 @@ intros. case (Z_le_dec a x); intro. case (Z_le_dec x b); intro.
 left. auto. right. intros [h1 h2]. contradiction.
 right. intros [h1 h2]. contradiction.
 Defined.
+
+(****************************************************************************)
 
 Definition nat_of_Z (x : Z) : nat :=
   match x with
@@ -38,3 +48,14 @@ Proof.
     intros _. rewrite Zpos_eq_Z_of_nat_o_nat_of_P. reflexivity.
     compute. intro n; case n; reflexivity.
 Qed.
+
+(****************************************************************************)
+
+Section update_map.
+
+Variables (A : Type) (eqdec : forall x y : A, {x=y}+{~x=y}) (B : Type).
+
+Definition update_map (a : A) (b : B) (f : A -> B) : A -> B :=
+  fun x => if eqdec x a then b else f x.
+
+End update_map.
