SemanticsPC.v
@@ -45,29 +45,24 @@ if ConditionPassed(cond) then
 
 Definition Adc (Sbit : bool) (Rd Rn : reg_num) (so : word) (s : state)
   (m : processor_mode) : result :=
-  let word_of_var (k : nat) : word :=
-    match k with
-      | 0 => Sbit
-      | 1 => Rd
-      | 2 => Rn
-      | 3 => so
-      | _ => dummy
-    end in
-  let Sbit := Var 0 in
-  let Rd := Var 1 in
-  let Rn := Var 2 in
-  let so := Var 3 in interp word_of_var m s
+  let env := assoc 0 Sbit (assoc 1 Rd (assoc 2 Rn (assoc 3 so empty))) in
+  let Sbit := Var 0 in let Rd := Var 1 in let Rn := Var 2 in let so := Var 3 in
+    interp env m s
     (IfThen ConditionPassed
-      (Seq (Affect (LReg Rd) (Add (Add (Reg Rn) so) (Flag Cbit)))
+      (Seq (Affect (Reg Rd) All (Add (Add (State (Reg Rn) All) so)
+                                     (State CPSR (Bit Cbit))))
         (IfThenElse (BAnd (Eq Sbit W1) (Eq Rd W15))
           Affect_CPSR_SPSR
           (IfThen (Eq Sbit W1)
-            (Seq (Affect (LFlag Nbit) (Bit 31 (Reg Rd)))
-              (Seq (Affect (LFlag Zbit) (If (Eq (Reg Rd) W0) W1 W0))
-                (Seq (Affect (LFlag Cbit)
-                  (CarryFrom_add3 (Reg Rn) so (Flag Cbit)))
-                (Affect (LFlag Vbit)
-                  (OverflowFrom_add3 (Reg Rn) so (Flag Cbit)))))))))).
+            (Seq (Affect CPSR (Bit Nbit) (State (Reg Rd) (Bit 31)))
+              (Seq (Affect CPSR (Bit Zbit)
+                           (If (Eq (State (Reg Rd) All) W0) W1 W0))
+                (Seq (Affect CPSR (Bit Cbit)
+                  (CarryFrom_add3 (State (Reg Rn) All) so
+                                  (State CPSR (Bit Cbit))))
+                (Affect CPSR (Bit Vbit)
+                  (OverflowFrom_add3 (State (Reg Rn) All) so
+                                     (State CPSR (Bit Cbit))))))))))).
 
 (****************************************************************************)
 (** A4.1.3 ADD (p. 156) *)
